Finish morphing

typing.v
@@ -15,21 +15,177 @@ Inductive Wt {n m} (Γ : context n m) : tm n m -> ty m -> Prop :=
 | T_Var i :
   (* ----------- *)
   Wt Γ (var_tm i) (Γ i)
+
 | T_Abs A a B :
   Wt (A .: Γ) a B ->
   (* ----------------- *)
   Wt Γ (Lam A a) (Fun A B)
+
 | T_App a A B b :
   Wt Γ a (Fun A B) ->
   Wt Γ b A ->
+  (* ---------- *)
   Wt Γ (App a b) B
+
 | T_TAbs a A :
   Wt (Γ >> ren_ty shift) a A ->
+  (* ------------------------ *)
   Wt Γ (TLam a) (Forall A)
+
 | T_TApp a A B :
   Wt Γ a (Forall A) ->
+  (* ------------------------------ *)
   Wt Γ (TApp a B) (subst_ty (B..) A).
 
-Lemma renaming {n m}
+#[export]Hint Constructors Wt : core.
+
+Lemma T_TApp' {n m} (Γ : context n m) a A B0 B :
+  B0 = (subst_ty (B..) A) ->
+  Wt Γ a (Forall A) ->
+  Wt Γ (TApp a B) B0.
+Proof. qauto ctrs:Wt. Qed.
+
+Lemma T_Var' {n m} ( Γ : context n m) i A :
+  A = Γ i ->
+  (* ----------- *)
+  Wt Γ (var_tm i) A.
+Proof. move => *; subst; auto. Qed.
+
+Definition is_renaming {n m n' m'}
   (Γ : context n m)
-  (ξ : fin n -> )
+  (Δ : context n' m')
+  (ξ0 : fin n -> fin n')
+  (ξ1 : fin m -> fin m') :=
+  forall (i : fin n),
+    ren_ty ξ1 (Γ i) = Δ (ξ0 i).
+
+Definition is_renaming_lam_ext {n m n' m'}
+  (Γ : context n m)
+  (Δ : context n' m')
+  (ξ0 : fin n -> fin n')
+  (ξ1 : fin m -> fin m')
+  A :
+  is_renaming Γ Δ ξ0 ξ1 ->
+  is_renaming (A .: Γ) (ren_ty ξ1 A .: Δ) (upRen_tm_tm ξ0) (upRen_tm_ty ξ1).
+Proof. hauto lq:on rew:off inv:option unfold:is_renaming. Qed.
+
+Definition is_renaming_tlam_ext {n m n' m'}
+  (Γ : context n m)
+  (Δ : context n' m')
+  (ξ0 : fin n -> fin n')
+  (ξ1 : fin m -> fin m')
+  (h : is_renaming Γ Δ ξ0 ξ1) :
+  is_renaming (Γ >> ren_ty shift) (Δ >> ren_ty shift) (upRen_ty_tm ξ0) (upRen_ty_ty ξ1).
+Proof.
+  move : h.
+  rewrite /is_renaming => h i.
+  asimpl.
+  rewrite -h.
+  by asimpl.
+Qed.
+
+#[export]Hint Unfold is_renaming : core.
+#[export]Hint Resolve is_renaming_lam_ext : core.
+
+Lemma renaming {n m} a A
+  (Γ : context n m)
+  (h : Wt Γ a A) :
+  forall n' m'
+  (ξ0 : fin n -> fin n')
+  (ξ1 : fin m -> fin m')
+  (Δ : context n' m'),
+  is_renaming Γ Δ ξ0 ξ1 ->
+  Wt Δ (ren_tm ξ0 ξ1 a) (ren_ty ξ1 A).
+Proof.
+  elim : n m Γ a A / h.
+  - hauto lq:on ctrs:Wt unfold:is_renaming.
+  - move => * /=; eauto using is_renaming_lam_ext.
+  - hauto q:on ctrs:Wt.
+  - move => * /=; eauto using is_renaming_tlam_ext.
+  - move => * /=.
+    apply : T_TApp'; eauto.
+    by asimpl.
+Qed.
+
+Lemma weakening_tm {n m} a A
+  (Γ : context n m)
+  (h : Wt Γ a A)
+  (B : ty m) :
+  Wt (B .: Γ) (ren_tm shift id a) A.
+Proof.
+  replace A with (ren_ty id A); last by asimpl.
+  apply renaming with (Γ := Γ); auto.
+  rewrite /is_renaming => i.
+  by asimpl.
+Qed.
+
+Definition is_morphing {n m n' m'}
+  (Γ : context n m)
+  (Δ : context n' m')
+  (ξ0 : fin n -> tm n' m')
+  (ξ1 : fin m -> ty m') :=
+  forall (i : fin n),
+    Wt Δ (ξ0 i) (subst_ty ξ1 (Γ i)).
+
+Lemma up_tm_ty_is_id {n m}
+  (ξ : fin n -> ty m) :
+  up_tm_ty ξ = ξ.
+  by asimpl. Qed.
+
+Definition is_morphing_lam_ext {n m n' m'}
+  (Γ : context n m)
+  (Δ : context n' m')
+  (ξ0 : fin n -> tm n' m')
+  (ξ1 : fin m -> ty m')
+  A :
+  is_morphing Γ Δ ξ0 ξ1 ->
+  is_morphing (A .: Γ) (subst_ty ξ1 A .: Δ) (up_tm_tm ξ0) ξ1.
+Proof.
+  rewrite /is_morphing => h.
+  destruct i as [i|].
+  - simpl.
+    asimpl.
+    eauto using weakening_tm.
+  - asimpl.
+    simpl.
+    apply T_Var'; by asimpl.
+Qed.
+
+Definition is_morphing_tlam_ext {n m n' m'}
+  (Γ : context n m)
+  (Δ : context n' m')
+  (ξ0 : fin n -> tm n' m')
+  (ξ1 : fin m -> ty m') :
+  is_morphing Γ Δ ξ0 ξ1 ->
+  is_morphing (Γ >> ren_ty shift) (Δ >> ren_ty shift) (up_ty_tm ξ0) (up_ty_ty ξ1).
+Proof.
+  rewrite /is_morphing => h i.
+  asimpl.
+  move /(_ i) in h.
+  apply renaming with (ξ0 := id) (ξ1 := shift) (Δ := Δ >> ren_ty shift) in h;
+    [by asimpl in h | sfirstorder unfold:is_renaming].
+Qed.
+
+Lemma morphing {n m} a A
+  (Γ : context n m)
+  (h : Wt Γ a A) :
+  forall n' m'
+    (ξ0 : fin n -> tm n' m')
+    (ξ1 : fin m -> ty m')
+    (Δ : context n' m'),
+    is_morphing Γ Δ ξ0 ξ1 ->
+    Wt Δ (subst_tm ξ0 ξ1 a) (subst_ty ξ1 A).
+Proof.
+  elim : n m Γ a A / h.
+  - sfirstorder unfold:is_morphing ctrs:Wt.
+  - move => n m Γ A a B h0 ih0 * /=.
+    apply T_Abs.
+    rewrite up_tm_ty_is_id.
+    eauto using is_morphing_lam_ext.
+  - hauto q:on ctrs:Wt.
+  - move => n m Γ a A h0 ih0 n' m' ξ0 ξ1 Δ hξ /=.
+    apply T_TAbs.
+    eauto using is_morphing_tlam_ext.
+  - move => * /=.
+    apply : T_TApp'; eauto; by asimpl.
+Qed.
